Wasm/AuxDefs.lean
@@ -1,0 +1,37 @@
+import Std
+import Mathlib.Data.List.Basic
+
+theorem Nat.lt_left_add {a b c : Nat} (h₁ : a + b < c) : a < c := by
+  induction b with
+  | zero => exact h₁
+  | succ n ih =>
+    have h₂ := Nat.lt_succ_of_lt h₁
+    rw [Nat.add_succ] at h₂
+    have h₃ := Nat.lt_of_succ_lt_succ h₂
+    apply ih h₃
+
+theorem Nat.lt_add_left {a b c : Nat} (h : a + b < c) : b < c := by
+  rw [Nat.add_comm] at h
+  apply lt_left_add h
+
+
+theorem Nat.le_trans_lt {a b c : Nat} (h₁ : a ≤ b) (h₂ : b < c) : a < c := by
+  cases h₁ with
+  | refl   => exact h₂
+  | step h => apply Nat.lt_trans (Nat.lt_succ_of_le h) h₂
+
+theorem Nat.two_pow_succ_pred : Nat.succ (Nat.pred (2 ^ n)) = 2 ^ n :=
+  Nat.lt_iff_le_and_ne.mp (Nat.pos_pow_of_pos n (Nat.zero_lt_succ 1))
+    |>.right
+    |>.symm
+    |> Nat.succ_pred
+
+theorem Nat.zero_lt_two_pow {n : Nat} : 0 < 2 ^ n := by
+  exact Nat.pos_pow_of_pos n ((Nat.zero_lt_succ 1))
+
+theorem List.length_ofFn {f : Fin n → α} : List.length (List.ofFn f) = n := by
+  simp [List.ofFn]
+
+
+def String.concatWith [ToString α] (str : String) (list : List α) : String :=
+  String.intercalate str (list.map toString)
