Wasm/Binary/Index.lean
@@ -1,0 +1,53 @@
+import Wasm.Binary.Opcode
+import Wasm.Syntax.Index
+open Numbers
+
+namespace Wasm.Binary.Module.Index
+
+open Wasm.Syntax.Module.Index
+
+instance : Opcode Typ      := ⟨toOpcode ∘ cast (by unfold Typ     ; rfl),
+  fun x => do
+    let resb ← ofOpcode x
+    return (cast (by unfold Typ     ; rfl) resb.1, resb.2)
+  ⟩
+instance : Opcode Function := ⟨toOpcode ∘ cast (by unfold Function; rfl),
+  fun x => do
+    let resb ← ofOpcode x
+    return (cast (by unfold Function; rfl) resb.1, resb.2)
+  ⟩
+instance : Opcode Table    := ⟨toOpcode ∘ cast (by unfold Table   ; rfl),
+  fun x => do
+    let resb ← ofOpcode x
+    return (cast (by unfold Table   ; rfl) resb.1, resb.2)
+  ⟩
+instance : Opcode Memory   := ⟨toOpcode ∘ cast (by unfold Memory  ; rfl),
+  fun x => do
+    let resb ← ofOpcode x
+    return (cast (by unfold Memory; rfl) resb.1, resb.2)
+  ⟩
+instance : Opcode Global   := ⟨toOpcode ∘ cast (by unfold Global  ; rfl),
+  fun x => do
+    let resb ← ofOpcode x
+    return (cast (by unfold Global  ; rfl) resb.1, resb.2)
+  ⟩
+instance : Opcode Element  := ⟨toOpcode ∘ cast (by unfold Element ; rfl),
+  fun x => do
+    let resb ← ofOpcode x
+    return (cast (by unfold Element ; rfl) resb.1, resb.2)
+  ⟩
+instance : Opcode Data     := ⟨toOpcode ∘ cast (by unfold Data    ; rfl),
+  fun x => do
+    let resb ← ofOpcode x
+    return (cast (by unfold Data    ; rfl) resb.1, resb.2)
+  ⟩
+instance : Opcode Local    := ⟨toOpcode ∘ cast (by unfold Local   ; rfl),
+  fun x => do
+    let resb ← ofOpcode x
+    return (cast (by unfold Local   ; rfl) resb.1, resb.2)
+  ⟩
+instance : Opcode Label    := ⟨toOpcode ∘ cast (by unfold Label   ; rfl),
+  fun x => do
+    let resb ← ofOpcode x
+    return (cast (by unfold Label   ; rfl) resb.1, resb.2)
+  ⟩
