Wasm/Binary/Opcode.lean
@@ -1,10 +1,52 @@
-namespace Wasm
+import Wasm.Util
+import Wasm.Syntax.Value
+import Numbers
+open Numbers
 
-class ToOpcode (α : Type u) where
-  toOpcode : α → UInt8
+namespace Wasm.Binary
 
-instance {α} [ToOpcode α] : ToOpcode (id α) :=
-  inferInstanceAs (ToOpcode α)
+abbrev Byte    := UInt8
+abbrev ByteSeq := List Byte -- maybe change : )
 
-instance {α} [ToOpcode α] : ToOpcode (Id α) :=
-  inferInstanceAs (ToOpcode α)
+def Byte.toSeq : UInt8 → List UInt8 := (.cons · [])
+
+instance : Coe Byte ByteSeq := ⟨Byte.toSeq⟩
+
+class Opcode (α : Type u) where
+  toOpcode : α → ByteSeq
+  ofOpcode : ByteSeq → Option (α × ByteSeq)
+
+export Opcode (toOpcode ofOpcode)
+
+instance {α} [Opcode α] : Opcode (id α) := inferInstanceAs (Opcode α)
+instance {α} [Opcode α] : Opcode (Id α) := inferInstanceAs (Opcode α)
+
+-- todo: use Unsigned stuff
+instance : Opcode (Unsigned n) := ⟨sorry, sorry⟩
+instance : Opcode (Signed n)   := ⟨sorry, sorry⟩
+instance : Opcode Nat          := ⟨sorry, sorry⟩
+instance : Opcode (Wasm.Syntax.Value.FloatN nn) := ⟨sorry, sorry⟩
+
+nonrec def List.toOpcode [Opcode α] (list : List α) : ByteSeq :=
+  toOpcode list.length ++ (list.map toOpcode).join
+
+nonrec def Vec.toOpcode [Opcode α] (vec : Vec α) : ByteSeq :=
+  toOpcode vec.length ++ (vec.list.map toOpcode).join
+
+nonrec def Vec.ofOpcode [Opcode α] (bytes : ByteSeq)
+    : Option (Vec α × ByteSeq) := do
+  let lenbytes : Unsigned32 × ByteSeq ← ofOpcode bytes
+
+  let mut vec := Vec.nil
+  let mut bytes := lenbytes.2
+  for i in [:lenbytes.1.toNat] do
+    let valbytes : α × ByteSeq ← ofOpcode bytes
+    bytes := valbytes.2
+
+    vec := Vec.cons valbytes.1 vec (by
+        sorry
+      )
+
+  return (vec.reverse, bytes)
+
+instance [Opcode α] : Opcode (Vec α) := ⟨Vec.toOpcode, Vec.ofOpcode⟩
