Wasm/Binary/Typ.lean
@@ -5,34 +5,129 @@ import Wasm.Util
 import Wasm.Binary.Opcode
 import Wasm.Syntax.Typ
 
-namespace Wasm.Syntax.Typ
+namespace Wasm.Binary.Typ
+
+open Wasm.Syntax.Typ
 
 def Num.toOpcode : Num → UInt8
   | .i32 => 0x7F
   | .i64 => 0x7E
   | .f32 => 0x7D
   | .f64 => 0x7C
-instance : ToOpcode Num := ⟨Num.toOpcode⟩
+
+def Num.ofOpcode : ByteSeq → Option (Num × ByteSeq)
+  | 0x7F :: rest => .some (.i32, rest)
+  | 0x7E :: rest => .some (.i64, rest)
+  | 0x7D :: rest => .some (.f32, rest)
+  | 0x7C :: rest => .some (.f64, rest)
+  | _            => .none
+
+instance : Opcode Num := ⟨Byte.toSeq ∘ Num.toOpcode, Num.ofOpcode⟩
+
 
 def Vec.toOpcode : Syntax.Typ.Vec → UInt8
   | .v128 => 0x7B
-instance : ToOpcode Syntax.Typ.Vec := ⟨Vec.toOpcode⟩
+
+def Vec.ofOpcode : ByteSeq → Option (Syntax.Typ.Vec × ByteSeq)
+  | 0x7B :: rest => .some  (.v128, rest)
+  | _            => .none
+
+instance : Opcode Syntax.Typ.Vec := ⟨Byte.toSeq ∘ Vec.toOpcode, Vec.ofOpcode⟩
+
 
 def Ref.toOpcode : Ref → UInt8
   | .func   => 0x70
   | .extern => 0x6F
-instance : ToOpcode Ref := ⟨Ref.toOpcode⟩
+
+def Ref.ofOpcode : ByteSeq → Option (Ref × ByteSeq)
+  | 0x70 :: rest => .some  (.func, rest)
+  | 0x6F :: rest => .some  (.extern, rest)
+  | _            => .none
+
+instance : Opcode Ref := ⟨Byte.toSeq ∘ Ref.toOpcode, Ref.ofOpcode⟩
+
 
 def Val.toOpcode : Val → UInt8
-  | .num v => v.toOpcode
-  | .vec v => v.toOpcode
-  | .ref v => v.toOpcode
-instance : ToOpcode Val := ⟨Val.toOpcode⟩
+  | .num v => Num.toOpcode v
+  | .vec v => Vec.toOpcode v
+  | .ref v => Ref.toOpcode v
 
--- todo Result + Func
+def Val.ofOpcode (seq : ByteSeq) : Option (Val × ByteSeq) :=
+      (do (← Num.ofOpcode seq).map Val.num id)
+  <|> (do (← Vec.ofOpcode seq).map Val.vec id)
+  <|> (do (← Ref.ofOpcode seq).map Val.ref id)
 
--- todo Limit + Mem + Table
+instance : Opcode Val := ⟨Byte.toSeq ∘ Val.toOpcode, Val.ofOpcode⟩
 
--- todo Global
+
+def Result.toOpcode (res : Result) : ByteSeq := Wasm.Binary.Vec.toOpcode res
+def Result.ofOpcode (seq : ByteSeq) : Option (Result × ByteSeq) :=
+  Wasm.Binary.Vec.ofOpcode seq
+instance : Opcode Result := ⟨Result.toOpcode, Result.ofOpcode⟩
+
+
+nonrec def Func.toOpcode (func : Func) : ByteSeq :=
+  0x60 :: toOpcode func.args ++ toOpcode func.result
+
+def Func.ofOpcode : ByteSeq → Option (Func × ByteSeq)
+  | 0x60 :: rest => do
+    let argsb ← Wasm.Binary.Vec.ofOpcode rest
+    let resb ← Wasm.Binary.Vec.ofOpcode argsb.2
+    return (⟨argsb.1, resb.1⟩, resb.2)
+  | _ => .none
+
+instance : Opcode Func := ⟨Func.toOpcode, Func.ofOpcode⟩
+
+
+nonrec def Limit.toOpcode (lim : Limit) : ByteSeq :=
+  match lim.max with
+  | .none   => 0x00 :: toOpcode lim.min
+  | .some m => 0x01 :: toOpcode lim.min ++ toOpcode m
+
+nonrec def Limit.ofOpcode : ByteSeq → Option (Limit × ByteSeq)
+  | 0x00 :: rest => do
+    let minb : Unsigned32 × ByteSeq ← ofOpcode rest
+    return (⟨minb.1, .none⟩, minb.2)
+  | 0x01 :: rest => do
+    let minb : Unsigned32 × ByteSeq ← ofOpcode rest
+    let maxb : Unsigned32 × ByteSeq ← ofOpcode minb.2
+    return (⟨minb.1, .some maxb.1⟩, maxb.2)
+  | _ => .none
+
+instance : Opcode Limit := ⟨Limit.toOpcode, Limit.ofOpcode⟩
+instance : Opcode Mem   := ⟨Limit.toOpcode, Limit.ofOpcode⟩
+
+
+nonrec def Table.toOpcode (tab : Table) : ByteSeq :=
+  toOpcode tab.2 ++ toOpcode tab.1
+
+nonrec def Table.ofOpcode (bytes : ByteSeq) : Option (Table × ByteSeq) := do
+  let refb ← Ref.ofOpcode bytes
+  let limb ← Limit.ofOpcode refb.2
+  return ((limb.1, refb.1), limb.2)
+
+instance : Opcode Table := ⟨Table.toOpcode, Table.ofOpcode⟩
+
+def Mut.toOpcode : Mut → Byte
+  | .const => 0x00
+  | .var   => 0x01
+
+def Mut.ofOpcode : ByteSeq → Option (Mut × ByteSeq)
+  | 0x00 :: rest => .some (.const, rest)
+  | 0x01 :: rest => .some (.var, rest)
+  | _            => .none
+
+instance : Opcode Mut := ⟨Byte.toSeq ∘ Mut.toOpcode, Mut.ofOpcode⟩
+
+
+nonrec def Global.toOpcode (g : Global) : ByteSeq :=
+  toOpcode g.2 ++ toOpcode g.1
+
+nonrec def Global.ofOpcode (bytes : ByteSeq) : Option (Global × ByteSeq) := do
+  let valb ← ofOpcode bytes
+  let mutb ← ofOpcode valb.2
+  return ((mutb.1, valb.1), mutb.2)
+
+instance : Opcode Global := ⟨Global.toOpcode, Global.ofOpcode⟩
 
 -- todo Extern
