Wasm/Util.lean
@@ -1,14 +1,8 @@
 import Std
 import Mathlib.Data.List.Basic
+import Wasm.AuxDefs
 
 namespace Wasm
-
-def String.concatWith [ToString α] (c : String) : List α → String
-  | .nil => ""
-  | .cons x .nil => toString x
-  | .cons x (.cons y ys) =>
-    String.append (String.append (toString x) c) (concatWith c (.cons y ys))
-
 
 def Vec.max_length : Nat := Nat.pow 2 32
 
@@ -20,7 +14,7 @@ deriving DecidableEq
 namespace Vec
 
 nonrec def toString [ToString α] (v : Vec α) : String :=
-  String.concatWith " " v.list
+  String.intercalate " " (v.list.map toString)
 
 def nil : Vec α := ⟨[], by simp⟩
 def single : α → Vec α := (⟨[·], by simp⟩)
@@ -58,37 +52,11 @@ def map (f : α → β) (v : Vec α) : Vec β :=
     exact v.maxLen
   ⟩
 
+def reverse (v : Vec α) : Vec α := ⟨v.list.reverse, by simp [v.maxLen]⟩
+
 @[inline] def length (v : Vec α) := v.list.length
 @[inline] def get (v : Vec α) (i : Fin v.length) := v.list.get i
 @[inline] def set (v : Vec α) (i : Fin v.length) (x : α) : Vec α :=
   ⟨v.list.set i x, by rw [List.length_set]; exact v.maxLen⟩
 
 end Vec
-
-theorem lt_left_add {a b c : Nat} (h₁ : a + b < c) : a < c := by
-  induction b with
-  | zero => exact h₁
-  | succ n ih =>
-    have h₂ := Nat.lt_succ_of_lt h₁
-    rw [Nat.add_succ] at h₂
-    have h₃ := Nat.lt_of_succ_lt_succ h₂
-    apply ih h₃
-
-theorem lt_add_left {a b c : Nat} (h : a + b < c) : b < c := by
-  rw [Nat.add_comm] at h
-  apply lt_left_add h
-
-
-theorem le_trans_lt {a b c : Nat} (h₁ : a ≤ b) (h₂ : b < c) : a < c := by
-  cases h₁ with
-  | refl   => exact h₂
-  | step h => apply Nat.lt_trans (Nat.lt_succ_of_le h) h₂
-
-theorem two_pow_succ_pred : Nat.succ (Nat.pred (2 ^ n)) = 2 ^ n :=
-  Nat.lt_iff_le_and_ne.mp (Nat.pos_pow_of_pos n (Nat.zero_lt_succ 1))
-    |>.right
-    |>.symm
-    |> Nat.succ_pred
-
-theorem zero_lt_two_pow {n : Nat} : 0 < 2 ^ n := by
-  exact Nat.pos_pow_of_pos n ((Nat.zero_lt_succ 1))
